\documentclass{article}

\usepackage{fancyhdr}
\usepackage[parfill]{parskip}
\usepackage{amssymb,amsmath}

\pagestyle{fancyplain}

\author{Todd Davies}
\title{Assignment 1 submission}
\date{\today}

\begin{document}

\rhead{Assignment 1 submission}
\lhead{\today}

\maketitle

\section*{Question 1}

The binary operation $*$ is defined on the set $\mathbb{Q}$ of rational numbers by:

\[
    p * q = 2p + 2q - pq - 2
\]

\subsection*{Part a}

Proof of commutativity:

\[
    \begin{split}
    p * q &= 2p + 2q - pq -2\\
          &= 2q + 2p - qp - 2\\
          &= q * p
    \end{split}
\]

\subsection*{Part b}

Proof of associativity:

\[
    \begin{split}
    (p * q) * r &= (2p + 2q - pq -2) * r\\
                &= 4p + 4q - 2pq - 4 + 2r - 2pr - 2qr + rpq + 2r - 2\\
                &= 4p + 4q - 2pq + 4r - 2pr - 2qr + rpq - 6\\
                &= 4r + 4q - 2pq - 4 + 2p - 2qp - 2rp + pqr + 2p -2\\
                &= (2r + 2q - rq - 2) * p\\
                &= (r * q) * p
    \end{split}
\]

\newpage

\section*{Question 2}

A small formal language {\it R} of expressions is defined by the following rules:
\begin{itemize}

    \item Each of the lower case letter symbols (from $a$ to $z$) is an expression.
    \item If $A$ is an expression, then so is $A!$
    \item If $A$ and $B$ are expressions then so are $AB\circledcirc$, $AB\circleddash$ and $AB\circledast$.

\end{itemize}

Some examples of expressions in this language may be:

\begin{itemize}
    \item $a$
    \item $a!$
    \item $ab\circledcirc$
    \item $ab!\circleddash$
    \item $abc\circledast\circledcirc$
\end{itemize}

See the attached sheet for the parse tree of the expression $np!q\circledcirc!rs\circleddash\circledast\circledcirc t\circleddash$:

\newpage

\section*{Question 3}

For any two subsets $A$ and $B$ of some set $S$,

\[
    (A \cup B) - (A \cap B) = (A - B) \cup (B - A)
\]

Where $X - Y = X \cap Y'$

\subsection*{Part a}

See attached sheet.

\subsection*{Part b}

Algebraic proof:

\[
    \begin{split}
    (A \cup B) - (A \cap B) &= (A \cup B) \cap (A \cap B)'\\
                            &= (A \cup B) \cap (A' \cup B')\\
                            &= ((A' \cup B') \cap A) \cup ((A' \cup B') \cap B)\\
                            &= ((A \cap A') \cup (A \cap B')) \cup ((B \cap A') \cup (B \cap B'))\\
                            &= (\emptyset \cup (A \cap B')) \cup ((B \cap A') \cup \emptyset)\\
                            &= (A \cap B') \cup (B \cap A')\\
                            &= (A - B) \cup (B - A)
    \end{split}    
\]

\end{document}
